deps/coq-poulet4/lib/Typed.v
@@ -1,5 +1,4 @@
 Require Import Coq.Numbers.BinNums.
-Require Petr4.String.
 Require Petr4.P4String.
 Require Petr4.P4Int.
 Require Import Coq.Classes.EquivDec.
